finished exercise 22

theories/type_systems/systemf/exercises03.v
@@ -4,52 +4,64 @@ From semantics.ts.systemf Require Import lang notation types tactics.
 
 (** Exercise 3 (LN Exercise 22): Universal Fun *)
 
+Definition Id: val :=
+  (Λ, (λ: "x", "x")).
+Definition Id_type : type :=
+  (∀: #0 → #0).
+Lemma Id_typed :
+  TY 0; ∅ ⊢ Id : Id_type.
+Proof. solve_typing. Qed.
+
 Definition fun_comp : val :=
-  #0 (* TODO *).
+  (Λ, Λ, Λ, (λ: "f" "g" "x", (App "g" (App "f" "x")))).
 Definition fun_comp_type : type :=
-  #0 (* TODO *).
+  (∀: ∀: ∀: ((#2 → #1) → (#1 → #0) → (#2 → #0))).
 Lemma fun_comp_typed :
   TY 0; ∅ ⊢ fun_comp : fun_comp_type.
 Proof. 
   (* should be solved by solve_typing. *)
-  (* TODO: exercise *)
-Admitted.
-
+  unfold fun_comp. unfold fun_comp_type.
+  solve_typing.
+Qed.
 
 Definition swap_args : val :=
-  #0 (* TODO *).
+  (Λ, Λ, Λ, (λ: "f" "a" "b", ("f" "b" "a"))).
 Definition swap_args_type : type :=
-  #0 (* TODO *).
+  (∀: ∀: ∀: (#2 → #1 → #0) → #1 → #2 → #0).
 Lemma swap_args_typed :
   TY 0; ∅ ⊢ swap_args : swap_args_type.
 Proof. 
   (* should be solved by solve_typing. *)
   (* TODO: exercise *)
-Admitted.
+  solve_typing.
+Qed.
 
 
 Definition lift_prod : val :=
-  #0 (* TODO *).
+  (Λ, Λ, Λ, Λ, (λ: "f" "g" "p", ("f" (Fst "p") , "g" (Snd "p")))).
 Definition lift_prod_type : type :=
-  #0 (* TODO *).
+  (∀: ∀: ∀: ∀: (#3 → #2) → (#1 → #0) → (#3 × #1) → (#2 × #0)).
 Lemma lift_prod_typed :
   TY 0; ∅ ⊢ lift_prod : lift_prod_type.
 Proof. 
   (* should be solved by solve_typing. *)
   (* TODO: exercise *)
-Admitted.
+  solve_typing.
+Qed.
 
 
 Definition lift_sum : val :=
-  #0 (* TODO *).
+  (Λ, Λ, Λ, Λ, (λ: "f" "g" "p", (Case "p" (λ: "x", InjL ("f" "x")) 
+    (λ: "x", InjR ("g" "x"))))).
 Definition lift_sum_type : type :=
-  #0 (* TODO *).
+  (∀: ∀: ∀: ∀: (#3 → #2) → (#1 → #0) → (Sum #3 #1) → (Sum #2 #0)).
 Lemma lift_sum_typed :
   TY 0; ∅ ⊢ lift_sum : lift_sum_type.
 Proof. 
   (* should be solved by solve_typing. *)
   (* TODO: exercise *)
-Admitted.
+  solve_typing.
+Qed.
 
 
 (** Exercise 5 (LN Exercise 18): Named to De Bruijn *)
